Change to full annotations.

skeletons/skeleton_lemmas.v
@@ -19,16 +19,16 @@ apply skeletons_ignore_csubtype in H. auto.
 Qed.
 
 
-Fixpoint skeleton_val_type Γ v A (types : has_vtype Γ v A) {struct types}:
+Fixpoint skeleton_val_types Γ v A (types : has_vtype Γ v A) {struct types}:
   has_sk_vtype (skeletize_ctx Γ) (skeletize_val v) (skeletize_vtype A)
-with skeleton_comp_type Γ c C (types : has_ctype Γ c C) {struct types}:
+with skeleton_comp_types Γ c C (types : has_ctype Γ c C) {struct types}:
   has_sk_ctype (skeletize_ctx Γ) (skeletize_comp c) (skeletize_ctype C)
-with skeleton_hcases_type Γ h Σ D (types : has_htype Γ h Σ D) {struct types}:
+with skeleton_hcases_types Γ h Σ D (types : has_htype Γ h Σ D) {struct types}:
   has_sk_htype (skeletize_ctx Γ) (skeletize_hcases h) (skeletize_ctype D).
 Proof.
-all: rename skeleton_val_type into VL.
-all: rename skeleton_comp_type into CL.
-all: rename skeleton_hcases_type into HL.
+all: rename skeleton_val_types into VL.
+all: rename skeleton_comp_types into CL.
+all: rename skeleton_hcases_types into HL.
 {
 destruct types. destruct H1; simpl.
 + apply SkTypeUnit.
@@ -89,3 +89,33 @@ destruct types. destruct H2; simpl.
 }
 Qed.
 
+
+
+Fixpoint skeleton_val_unique_type Γ v A1 A2 
+  (types1 : has_sk_vtype Γ v A1) (types2 : has_sk_vtype Γ v A2) {struct v}:
+  A1 = A2
+with skeleton_comp_unique_type Γ c C1 C2 
+  (types1 : has_sk_ctype Γ c C1) (types2 : has_sk_ctype Γ c C2) {struct c}:
+  C1 = C2
+with skeleton_hcases_unique_type Γ h D1 D2 
+  (types1 : has_sk_htype Γ h D1) (types2 : has_sk_htype Γ h D2) {struct h}:
+  D1 = D2.
+Proof.
+{
+destruct v; inv types1; inv types2; eauto.
++ rewrite H1 in H2. inv H2. auto.
++ f_equal; eauto.
++ f_equal; eauto.
++ f_equal; eauto.
+}{
+destruct c; inv types1; inv types2; eauto.
++ f_equal; eauto.
++ apply (skeleton_val_unique_type _ _ _ _ H2) in H3. inv H3. eauto.
++ apply (skeleton_val_unique_type _ _ _ _ H3) in H4. inv H4. eauto.
++ apply (skeleton_val_unique_type _ _ _ _ H2) in H3. inv H3. eauto.
++ apply (skeleton_comp_unique_type _ _ _ _ H2) in H3. inv H3. eauto.
++ apply (skeleton_val_unique_type _ _ _ _ H2) in H3. inv H3. eauto.
+}{
+destruct h; inv types1; inv types2; eauto.
+}
+Qed.
