type_system/type_lemmas.v
@@ -46,45 +46,50 @@ Theorem preservation Γ c c' C:
   has_ctype Γ c C -> step c c' -> has_ctype Γ c' C.
 Proof.
 intros orig step. revert C orig. 
-induction step; intros C orig.
+induction step; intros C' orig.
 all: try unfold c_subs2_out.
 + apply shape_prodmatch in orig. destruct orig as [A [B [pair]]].
   apply shape_pair in pair. destruct pair.
   eapply c_subs_out_typesafe. eapply c_subs_out_typesafe.
   all: eauto. inv H0. apply v_shift_typesafe; auto.
 + apply shape_summatch in orig.
-  destruct orig as [A [B [vty [Left _]]]].
-  eapply c_subs_out_typesafe. exact Left. apply shape_left in vty. auto.
+  destruct orig as [A' [B' [vty [l _]]]].
+  eapply c_subs_out_typesafe. eauto. eapply shape_left in vty. 2: reflexivity.
+  destruct vty. inv H0. inv l. inv H0. 
+  apply TypeV; auto. eapply TypeVSubsume; eauto.
 + apply shape_summatch in orig.
-  destruct orig as [A [B [vty [_ Right]]]].
-  eapply c_subs_out_typesafe. exact Right. apply shape_right in vty. auto.
+  destruct orig as [A' [B' [vty [_ r]]]].
+  eapply c_subs_out_typesafe. eauto. eapply shape_right in vty. 2: reflexivity.
+  destruct vty. inv H0. inv r. inv H0. 
+  apply TypeV; auto. eapply TypeVSubsume; eauto.
 + apply shape_listmatch in orig.
-  destruct orig as [A[_[ty1 _]]]. auto.
+  destruct orig as [A'[_[ty1 _]]]. auto.
 + apply shape_listmatch in orig. destruct orig as [A[vty[_ ty2]]]. 
   apply shape_cons in vty. destruct vty as [vty vsty].  
   eapply c_subs_out_typesafe; eauto. eapply c_subs_out_typesafe; eauto.
   eapply v_shift_typesafe; eauto. inv vty. auto.
-+ apply shape_app in orig. destruct orig as [A [f]].
++ apply shape_app in orig. destruct orig.
   eapply c_subs_out_typesafe; eauto.
-+ apply shape_letrec in orig. destruct orig as [A [C' [c1ty]]].
++ eapply shape_letrec_full in orig. 2: reflexivity.
+  destruct orig as [c1ty c2ty].
   eapply c_subs_out_typesafe; eauto. apply TypeV. inv c1ty.
-  inv H. inv H3. auto. inv H. inv H0. auto.  
+  inv H. inv H4. auto. inv c2ty. inv H. auto. 
   apply TypeFun. apply TypeC. 
-  - inv c1ty. inv H0. auto.
+  - inv c1ty. inv H. auto.
   - inv c1ty. auto.
-  - eapply TypeLetRec. 2: exact c1ty.
-    assert (CtxU (CtxU (CtxU Γ A) A) (TyFun A C') 
-      = ctx_insert (CtxU (CtxU Γ A) (TyFun A C')) 2 A)
+  - eapply TypeLetRec; auto.
+    assert (CtxU (CtxU (CtxU Γ A) A) (TyFun A C) 
+      = ctx_insert (CtxU (CtxU Γ A) (TyFun A C)) 2 A)
     as insertion. { simpl. destruct Γ; auto. }
     rewrite insertion. apply c_insert_typesafe. auto.
-    inv H. inv H0. inv H5. auto.
-+ destruct C as (A, Σ, E) eqn:e. apply shape_do in orig.
+    inv c2ty. inv H. inv H5. auto.
++ destruct C' as (A, Σ, E) eqn:e. apply shape_do in orig.
   destruct orig as [A' [c1ty]].
   apply TypeC. inv c1ty. 3 : eapply TypeDo. all: eauto. inv H. auto.
-+ destruct C as (A, Σ, E) eqn:e. apply shape_do in orig.
++ destruct C' as (A, Σ, E) eqn:e. apply shape_do in orig.
   destruct orig as [A' [c1ty]]. eapply c_subs_out_typesafe. eauto.
   apply shape_ret in c1ty. auto.
-+ destruct C as (Ac, Σ, E) eqn:e. apply shape_do in orig.
++ destruct C' as (Ac, Σ, E) eqn:e. apply shape_do in orig.
   destruct orig as [A' [c1ty]]. eapply shape_op_full in c1ty; eauto.
   destruct c1ty as [vty[cty[Aop[Bop[gets[stya styb]]]]]]. apply TypeC.
   - inv vty. auto.
@@ -98,34 +103,35 @@ all: try unfold c_subs2_out.
       { simpl. destruct Γ; auto. }
       rewrite same. apply c_insert_typesafe. auto.
       inv cty. inv H0. auto.
-+ eapply shape_handle in orig. destruct orig as [C' [hty]]. 
++ eapply shape_handle in orig. destruct orig as [C [hty]]. 
   apply TypeC. inv hty. auto. inv hty. inv H1. auto.
   eapply TypeHandle; eauto.
-+ eapply shape_handle in orig. rename C into D. destruct orig as [C[hty]].
-  destruct C as (A, Σ, E). eapply shape_handler in hty as hty'. 
-  destruct hty' as [Σ'[D'[retty[hcty[r[st]]]]]]. eapply shape_ret in H.
++ eapply shape_handle in orig. rename C' into D. destruct orig as [C[hty]].
+  destruct C as (A', Σ, E). eapply shape_handler in hty as hty'. 
+  destruct hty' as [Σ'[D'[retty[hcty[r[sta[sty csty]]]]]]]. eapply shape_ret in H.
   eapply c_subs_out_typesafe; eauto. apply TypeC. 
   - inv H. apply WfCtxU; auto.
-  - inv hty. inv H2. auto.
-  - eapply TypeCSubsume; eauto.
-+ eapply shape_handle in orig. rename C into D. 
+  - inv hty. inv H1. auto.
+  - eapply TypeCSubsume; eauto. inv H.
+    eapply ctx_subtype_ctype; eauto; apply WfCtxU || apply STyCtxU; auto.
+    apply ctx_subtype_refl. auto.
++ eapply shape_handle in orig. rename C' into D. 
   destruct orig as [C[hty]]. destruct C as (Ac, Σ, E).
   eapply shape_handler in hty as hty'.
-  destruct hty' as [Σ'[D'[retty[hcty[r[st]]]]]].
+  destruct hty' as [Σ'[D'[retty[hcty[r[sta[stysig styd]]]]]]].
   eapply shape_op_full in H0 as opt; eauto.
-  destruct opt as [vty[cty[Aop[Bop[gets[stya styb]]]]]].
+  destruct opt as [vty[cty[Aop'[Bop'[gets[stya styb]]]]]].
   assert (wf_ctx Γ) by (inv hty; auto). 
-  apply TypeC; auto. inv hty. inv H4. auto.
+  apply TypeC; auto. inv hty. inv H3. auto.
   eapply TypeCSubsume; eauto.
-  assert (wf_vtype A) as wfa by (inv vty; auto).
-  assert (wf_vtype B) as wfb by (inv cty; inv H3; auto).
+  assert (wf_vtype Aop) as wfa by (inv vty; auto).
+  assert (wf_vtype Bop) as wfb by (inv cty; inv H2; auto).
   assert (wf_ctype D') as wfd by (inv hcty; auto).
+  eapply c_subs_out_typesafe; eauto.
   eapply c_subs_out_typesafe.
-  instantiate (1:= A).
-  eapply c_subs_out_typesafe.
-  instantiate (1:= TyFun B D').
+  instantiate (1:= TyFun Bop D').
   - eapply sig_subtype_get_Some in gets; eauto.
-    destruct gets as [A'[B'[gets']]]. inv H3.
+    destruct gets as [A'[B'[gets']]]. inv H2.
     eapply ctx_subtype_ctype. eapply case_has_type; eauto.
     * apply WfCtxU. apply WfCtxU. 3: apply WfTyFun. all: auto.
     * apply STyCtxU. apply STyCtxU.
@@ -137,20 +143,20 @@ all: try unfold c_subs2_out.
     apply TypeV. auto. apply WfTyFun; auto.
     eapply TypeFun. apply TypeC. apply WfCtxU. all: auto.
     eapply TypeHandle. 2: eauto.
-    assert (CtxU Γ B = ctx_insert Γ 0 B) as same by (destruct Γ; simpl; auto).
+    assert (CtxU Γ Bop = ctx_insert Γ 0 Bop) as same.
+    { destruct Γ; simpl; auto. }
     rewrite same. eapply v_insert_typesafe. 2: auto.
     apply TypeV. auto. apply WfTyHandler. inv H0. auto. auto.
     assert (wf_sig Σ') as wfsig by (inv hcty; auto).
-    eapply TypeVSubsume. instantiate (1:=(TyHandler (CTy Ac Σ' E) D')).
-    * inv H0. inv H4.
+    eapply TypeVSubsume. instantiate (1:=(TyHandler (CTy A Σ' E) D')).
+    * inv H0. inv H3.
       apply TypeV. auto. apply WfTyHandler; auto. apply WfCTy; auto.
+      inv retty. inv H0. auto.
       eapply wf_eqs_sig_subtype; eauto. apply TypeHandler; auto.
-    * inv H0. inv H4.
-      apply STyHandler. apply STyCTy. 2: auto.
-      apply vsubtype_refl. inv cty. inv H4. auto.
+    * inv H0. inv H3.
+      apply STyHandler. apply STyCTy; auto.
       eapply eqs_subtype_refl; eauto.
       apply csubtype_refl. auto.
-  - auto.
 Qed.
 
 (* ==================== Progress ==================== *)
@@ -180,14 +186,16 @@ revert C. induction c; intros C orig.
   destruct shape. 2: destruct H0.
   - destruct H0 as [n same]. rewrite same in *.
     apply shape_var_ctx_empty in vty. destruct vty.
-  - destruct H0 as [v' [same]]. rewrite same. eexists. apply Step_MatchLeft.
-  - destruct H0 as [v' [same]]. rewrite same. eexists. apply Step_MatchRight.
+  - destruct H0 as [v'[A'[B'[same]]]].
+    rewrite same. eexists. apply Step_MatchLeft.
+  - destruct H0 as [v'[A'[B'[same]]]].
+    rewrite same. eexists. apply Step_MatchRight.
 + right. right.
   eapply shape_listmatch in orig. destruct orig as [A[vty[cty1 cty2]]].
-  eapply shape_list_full in vty as shape; eauto. destruct shape. 
+  eapply shape_list_full in vty as shape; eauto. destruct shape.
   destruct H as [n same]. subst. apply shape_var_ctx_empty in vty. destruct vty. 
   destruct H.
-  - exists c1. subst. apply Step_MatchNil.
+  - exists c1. destruct H. subst. apply Step_MatchNil.
   - destruct H as [w[ws[same[wty wsty]]]]. subst. 
     eexists. apply Step_MatchCons. 
 + right. right.
@@ -213,15 +221,15 @@ revert C. induction c; intros C orig.
   2: reflexivity. destruct shape.
   { destruct H0 as [n same]. subst.
     apply shape_var_ctx_empty in hty. contradiction. }
-  destruct H0 as [c_r[h[Σ'[D'[same[crty]]]]]]. subst.
+  destruct H0 as [c_r[h[A'[Σ'[D'[same[crty]]]]]]]. subst.
   destruct H'. 2: destruct H1.
   - destruct H1 as [v]. subst. eexists. apply Step_HandleRet.   
   - destruct H1 as [op[Aop[Bop[v[c']]]]]. subst.
-    destruct H0 as [hcsty[r[sigsty]]].
+    destruct H0 as [hcsty[r[stya[sigsty styd]]]].
     eapply shape_op_full in H; eauto.
     destruct H as [vty[cty[A_op[B_op[gets _]]]]].
     eapply sig_subtype_get_Some in gets. 2: exact sigsty.
-    destruct gets as [A'[B'[gets']]].
+    destruct gets as [A''[B''[gets']]].
     eapply h_has_case in hcsty. 2: exact gets'.
     destruct hcsty as [c_op finds].
     eexists. eapply Step_HandleOp. eauto.    
